Bedrock/Platform/Facade/CompileUnit2.v
@@ -1,0 +1,34 @@
+Set Implicit Arguments.
+
+Require Import StringMap.
+Require Import AxSpec.
+Require Import DFModule.
+Require Import String.
+Require Import StringMapFacts.
+Require Import Bedrock.Platform.Cito.NameDecoration.
+Require Import GLabelMap.
+Require Import ListFacts3.
+
+Section TopSection.
+
+  Variable ADTValue : Type.
+  (* exported axiomatic specs *)
+  Variable exports : StringMap.t (AxiomaticSpec ADTValue).
+
+  Record CompileUnit :=
+    {
+      module : DFModule ADTValue;
+      (* the name of the module that contains axiomatic export specs *)
+      ax_mod_name : string;
+      (* the name of the module that contains operational export specs *)
+      op_mod_name : string;
+      exports_in_domain : is_sub_domain exports (Funs module) = true;
+      op_mod_name_ok : is_good_module_name op_mod_name = true;
+      op_mod_name_not_in_imports :
+        let imported_module_names := List.map (fun x => fst (fst x)) (GLabelMap.elements (Imports module)) in
+        List.forallb (fun x => negb (string_bool op_mod_name x)) imported_module_names = true;
+      name_neq : negb (string_bool ax_mod_name op_mod_name) = true;
+      proof : True (* placeholder, to be filled in later *)
+    }.
+
+End TopSection.
